Using 'good' definition of less-or-equal

forcing/GRTT_SProp.v
@@ -8,36 +8,57 @@ Require Import List.
 
 (* Some axioms *)
 Require Import FunctionalExtensionality.
-Require Import ProofIrrelevance.
 
-Open Scope string.
+(* To be able to work with values in SProp we define boxing/unboxing *)
+Inductive sBox (A : SProp) : Prop := sbox : A -> sBox A.
 
-Inductive sle (n : nat) : nat -> SProp :=
-  sle_n : sle n n
-| sle_S : forall m : nat, sle n m -> sle n (S m).
+Definition ubox {A : SProp} (bA : sBox A) : A :=
+  match bA with
+    sbox _ X => X
+  end.
 
-
-Definition sle_n_Sm {n m : nat} : sle n m -> sle n (S m).
+(* All attempts use [rewrite] or [subst] fail, because [eq_sind_r] is not defined.
+   We define it, but for some reason the tactics still complain about [eq_sind_r] *)
+Definition eq_sind_r : forall (A : Type) (x : A) (P : A -> SProp),
+    P x -> forall y : A, y = x -> P y.
 Proof.
-  intros H. induction n; constructor; auto.
+  intros A x P H y Heq. apply ubox. subst. apply sbox. exact H.
 Defined.
+
+Inductive sle : nat -> nat -> SProp :=
+  sle_0 : forall n, sle 0 n
+| sle_S : forall n m : nat, sle n m -> sle (S n) (S m).
 
 Definition sle_refl (n : nat) : sle n n.
 Proof.
-  induction n;constructor.
+  induction n;constructor;auto.
 Defined.
 
-Definition sle_trans (n m p : nat) : sle n m -> sle m p -> sle n p.
+Definition sle_S_eq {n m} : sle (S n) (S m) -> sle n m.
 Proof.
-  intros f g. revert f.
-  induction g.
-  - intros. assumption.
-  - intros. constructor. apply IHg. assumption.
+  intros H.
+  inversion H. apply ubox. subst. apply sbox. exact H2.
 Defined.
+
+Definition sle_trans n m p (H : sle n m) (H': sle m  p) : sle n p.
+Proof.
+  revert H'. revert p. induction H.
+  - intros p H'. apply sle_0.
+  - intros p H'. inversion H'. apply ubox. subst. apply sbox. apply sle_S. apply IHsle;auto.
+Defined.
+
+(* This does not work, fails with the error:
+   Fixpoints on proof irrelevant inductive types should produce proof irrelevant
+   values.*)
+Fixpoint sle_trans' n m p (H : sle n m) (H': sle m  p) {struct H} : sle n p.
+Proof.
+  destruct H. apply sle_0.
+  inversion H'. apply ubox. subst. apply sbox. apply sle_S. exact (sle_trans _ _ _ H H1).
+Abort.
 
 Definition sle_Sn (n : nat) : sle n (S n).
 Proof.
-  constructor; apply sle_refl.
+  induction n; constructor; auto.
 Defined.
 
 Definition nat_obj : Type := nat.
@@ -51,20 +72,19 @@ Definition nat_comp (A B C : nat_obj) (g : B ≥ C) (f : A ≥ B) : nat_hom A C
   := sle_trans _ _ _ g f.
 Notation "f ∘ g" := (nat_comp _ _ _ f g) (at level 40).
 
-Definition Z_le_1 : sle 0 1 := sle_S _ _ (sle_n _).
+Arguments sbox {_}.
 
-Eval compute in (fun P Q (g : P ≥ Q) => g ∘ (# P)).
+(* Now, laws hold definitionally, thanks to SProp *)
+(* We use sbox'ed version to prove this *)
+Lemma nat_cat_left_id P R (g : R ≥ P)  : sbox (g ∘ (# _)) = sbox g.
+Proof. reflexivity. Qed.
 
-(* Now, laws hold definitionally *)
-(* Lemma nat_cat_left_id P R (g : R ≤ P)  : (g ∘ (# R)) = g. *)
-(* Proof. reflexivity. Qed. *)
+Lemma nat_cat_right_id P R (f : P ≥ R)  : sbox (f ∘ (# _)) = sbox f.
+Proof. reflexivity. Qed.
 
-(* Lemma nat_cat_right_id P R (f : P ≤ R)  : f ∘ (# R) = f. *)
-(* Proof. reflexivity. Qed. *)
-
-(* Lemma nat_cat_assoc P Q R S (f : P ≤ Q) (g : Q ≤ R) (h : R ≤ S): *)
-(*   f ∘ (g ∘ h) = (f ∘ g) ∘ h. *)
-(* Proof. reflexivity. Qed. *)
+Lemma nat_cat_assoc P Q R S (f : S ≥ Q) (g : R ≥ S) (h : P ≥ R):
+  sbox (f ∘ (g ∘ h)) = sbox ((f ∘ g) ∘ h).
+Proof. reflexivity. Qed.
 
 Quote Definition q_nat_obj := nat_obj.
 Quote Definition q_nat_hom := nat_hom.
@@ -74,14 +94,16 @@ Quote Definition q_nat_comp := nat_comp.
 Definition nat_cat : category :=
   mkCat q_nat_obj q_nat_hom q_id_nat_hom q_nat_comp.
 
-
 (* The definition of [later] operator *)
 
-Quote Definition qTypeConstr := (Type -> Type).
+(* Building required context to pass to the tranlation
+   Maybe, we should try to use the template monad here *)
 
-Check translate_type.
+
 Quote Recursively Definition q_def := nat_hom.
 Definition g_ctx := fst q_def.
+
+Quote Definition qTypeConstr := (Type -> Type).
 
 Definition tr_TypeConstr_syn :=
   Eval vm_compute in
@@ -91,15 +113,52 @@ Definition tr_TypeConstr_syn :=
 
 Import ListNotations.
 
-Make Definition gArrowTypeType := Eval vm_compute in (snd tr_TypeConstr_syn).
+Make Definition gTypeConstr := Eval vm_compute in (snd tr_TypeConstr_syn).
 
 Arguments nat_comp {_ _ _}.
 
-Definition later : gArrowTypeType.
+Definition later : gTypeConstr.
 Proof.
-  unfold gArrowTypeType.
+  unfold gTypeConstr.
   intros p T q f.
   destruct q.
   - apply unit.
   - apply (T q (sle_Sn q ∘ f) q (# _)).
 Defined.
+
+Quote Definition qType := Type.
+
+Definition tr_Type_syn :=
+  Eval vm_compute in
+    translate_type true None nil nat_cat
+                   {| Environ.env_globals := g_ctx|}
+                   tt qType.
+
+Make Definition gType := Eval vm_compute in (snd tr_Type_syn).
+
+Definition later_type (A : gType) : gType
+  := fun p q α => later p (fun p' _ q' => A p' q') q α.
+
+Notation "⊳ A" := (later_type A) (at level 40).
+
+Quote Definition qId := (fun (A : Type) => A).
+
+Definition tr_Arr_syn :=
+  Eval vm_compute in
+    translate true None nil nat_cat
+                   {| Environ.env_globals := g_ctx|}
+                   tt qId.
+
+(*A translation of [fun (x : Type) => x] from the original plugin *)
+Definition fooᶠ  : forall p : nat_obj,
+    (forall p0 : nat_obj, p ≥ p0 -> forall p1 : nat_obj, p0 ≥ p1 -> Type) ->
+    forall p0 : nat_obj, p ≥ p0 -> Type
+  := (fun (p : nat_obj) (x : forall p0 : nat_obj, p ≥ p0 -> forall p1 : nat_obj, p0 ≥ p1 -> Type) => x p (# _)).
+
+Make Definition gId :=
+  Eval vm_compute in (snd tr_Arr_syn).
+
+Lemma eq_gId_fooᶠ : gId = fooᶠ.
+Proof. reflexivity. Qed.
+
+(* Definition later_app : forall A B (t : ⊳ (A -> B)) (u : ⊳ A), ⊳ B. *)
